Lean4Lean/Tests.lean
@@ -8,6 +8,7 @@ import Lean4Lean.Tests.Toolchain
 import Lean4Lean.Tests.ConditionReflect
 import Lean4Lean.Tests.ModDivCondition
 import Lean4Lean.Tests.NatBitwise
+import Lean4Lean.Tests.NatBitwiseSpecializations
 import Lean4Lean.Tests.NatDiv
 import Lean4Lean.Tests.NatGcd
 import Lean4Lean.Tests.NatGcdProdState
